# Exercise 1.13

Prove that $Fib(n)$ is the closest integer to $\varphi^n / \sqrt{5}$, where
$\varphi=(1+\sqrt{5})/2$.

Hint: Let $\psi=(1-\sqrt{5})/2$. Use induction and the definition of the
Fibonacci numbers (see 1.2.2) to prove that
$Fib(n)=(\varphi^n âˆ’ \psi^n)/ \sqrt{5}$.

## Answer

Solving this exercise following the hint (proving [Binet's formula][binet] using
induction) is not so difficult. Some solutions are:

- https://sicp-solutions.net/post/sicp-solution-exercise-1-13/
- http://community.schemewiki.org/?sicp-ex-1.13

[binet]: https://en.wikipedia.org/wiki/Fibonacci_sequence#Binet's_formula

I have tried to solve this exercise without following that path. However, all
ideas leads that same destination: proving Binet's formula. Hence, I don't have
any better or worthy solution to document here.

Instead, I investigate on how can we derive the value of $\varphi$ and come up
with the [closed-form expression][cfe] (CFE from now on for short) of $Fib(n)$,
and document them instead.

[cfe]: https://en.wikipedia.org/wiki/Closed-form_expression

## Fibonacci sequence generalizations

### General starting points

Given a sequence $G(n)$ defined as:

$$
G(n) =
\begin{cases}
= a               & \text{if }  n = 0 \\
= b               & \text{if }  n = 1 \\
= G(n-1) + G(n-2) & \forall n > 1
\end{cases}
$$

One of such sequences is [Lucas numbers][lucas-num] where $a=2$ and $b=1$.

[lucas-num]: https://en.wikipedia.org/wiki/Lucas_number

We can check that

$$
\begin{split}
G(2) &= G(1) + G(0)      \\
     &= b + a            \\
G(3) &= G(2) + G(1)      \\
     &= (b + a) + a        \\
     &= b + 2a           \\
G(4) &= G(3) + G(2)      \\
     &= (b + 2a) + (b+a) \\
     &= 2b + 3a          \\
     &... \\
\end{split}
$$

Thus, we discover the relationship between $Fib(n)$ and $G(n)$.

$$
G(n) = a Fib(n) + b Fib(n-1) \tag{1}
$$

$(1)$ can be easily proved using induction. $(1)$ also means we can derive the
Closest-form expression of $G(n)$ from $Fib(n)$.

### Derive Binet's formula

People have found many ways to come up with the [golden ratio][golden] in the
formula. I'm document here the idea that I can fully understand with my high
school math knowledge, and might apply it in case I face similar problems.

[golden]: https://en.wikipedia.org/wiki/Golden_ratio

#### Intuitions

- Identify those important constants $\varphi$ and $\psi$, also note their
  properties (both are root of $x^2 = x+1$).
- Find relationship between them and $Fib(n)$, thus, derive the closest-form
  expression.
- Prove the formula using induction.

#### Find important constants

Examine the sequence $S(n) = \frac{Fib(n+1)}{Fib(n)}$, we can see that

- It alternates between $\gt L$ and $\lt L$.
- It converges to a specific value $L$, i.e. $S(n)$ is a convergent series.

<details>
  <summary>Code to generate the table</summary>

```racket
(printf "| n  | $Fib(n+1)/Fib(n)$ | Floating point | \n")
(printf "| -- | ----------------- | -------------- | \n")
(for ([n (in-range 4 10)])
  (define numerator (fib-iter (+ 1 n)))
  (define denominator (fib-iter n))
  (define v (/ numerator denominator))
  (printf "| ~a | ~a | ~a  |\n" n v (exact->inexact v)))
```

</details>

| n   | $Fib(n+1)/Fib(n)$ | Floating point     |
| --- | ----------------- | ------------------ |
| 2   | 2                 | 2.0                |
| 3   | 3/2               | 1.5                |
| 4   | 5/3               | 1.6666666666666667 |
| 5   | 8/5               | 1.6                |
| 6   | 13/8              | 1.625              |
| 7   | 21/13             | 1.6153846153846154 |
| 8   | 34/21             | 1.619047619047619  |
| 9   | 55/34             | 1.6176470588235294 |
| 10  | 89/55             | 1.6181818181818182 |
| 11  | 144/89            | 1.6179775280898876 |
| 12  | 233/144           | 1.6180555555555556 |
| 13  | 377/233           | 1.6180257510729614 |
| 14  | 610/377           | 1.6180371352785146 |
| 15  | 987/610           | 1.618032786885246  |
| 16  | 1597/987          | 1.618034447821682  |
| 17  | 2584/1597         | 1.6180338134001253 |
| 18  | 4181/2584         | 1.618034055727554  |
| 19  | 6765/4181         | 1.6180339631667064 |
| 20  | 10946/6765        | 1.6180339985218033 |

Here is how we can derive $L$.

$$
\begin{split}
\lim_{n\to\infty} S(n) &= \lim_{n\to\infty} \frac{Fib(n+1)}{Fib(n)}                 \\
                       &= \lim_{n\to\infty} 1 + \frac{Fib(n-1)}{Fib(n)}             \\
                       &= 1 + \lim_{n\to\infty} \frac{1}{\frac{Fib(n-1)}{Fib(n)}}   \\
                       &= 1 + \frac{1}{\lim_{n \to \infty} \frac{Fib(n-1)}{Fib(n)}} \\
                       &= 1 + \frac{1}{\lim_{n \to \infty} S(n)}                    \\
\end{split}
$$

That leads to

$$
L = 1 + \frac{1}{L} => L^2 = L + 1
$$

Solving that equation, we will get 2 values $\varphi$ and $\psi$, of which
$L = \varphi$.

$$
\begin{split}
\varphi & = \frac{1+\sqrt{5}}{2} \\
\psi    & = \frac{1-\sqrt{5}}{2}
\end{split}
$$

#### Derive the formula

Notice how $\varphi$ and $\psi$ satisfy these (easy to prove using induction,
albeit hard to come up):

$$
\begin{split}
\varphi^n & = Fib(n)\varphi + Fib(n-1) \\
\psi^n    & = Fib(n)\psi + Fib(n-1)
\end{split}
$$

From the 2 equations, we can compute $Fib(n)$ as

$$
\begin{split}
         & \varphi^n - \psi^n & = Fib(n) (\varphi - \psi)                 \\
=> \quad & Fib(n)             & = \frac{1}{\sqrt{5}}(\varphi^n - \psi^n)
\end{split}
$$

### Tribonacci

Let's consider a general Tribonacci sequence $GT(n)$.

$$
GT(n) =
\begin{cases}
a & \text{if } n = 0                           \\
b & \text{if } n = 1                           \\
c & \text{if } n = 2                           \\
GT(n-1) + GT(n-2) + GT(n-3) & \text{otherwise} \\
\end{cases}
$$

And the Tribonacci sequence $T(n)$ which is a specialized case of $GT(n)$ where
$a = b = 0$ and $c = 1$. First 10 values of $T(n)$ is below:

| $n$ | $T(n)$ |
| --- | ------ |
| 0   | 0      |
| 1   | 0      |
| 2   | 1      |
| 3   | 2      |
| 4   | 4      |
| 5   | 7      |
| 6   | 13     |
| 7   | 24     |
| 8   | 44     |
| 9   | 81     |
| 10  | 149    |

Once again, we can come up with the relationship between $GT(n)$ and $T(n)$
quite easy.

$$
\begin{split}
G(3)   & = G(2) + G(1) + G(0)                                                   \\
       & = c + b + a                                                            \\
G(4)   & = G(3) + G(2) + G(1)                                                   \\
       & = (c+b+a) + c + b                                                      \\
       & = 2c + 2b + a                                                          \\
G(5)   & = G(4) + G(3) + G(2)                                                   \\
       & = (2c + 2b + a) + (c + b + a) + c                                      \\
       & = 4c + 3b + 2a                     & = cT(4) + b(T(3) + T(2))  + aT(3) \\
G(6)   & = G(5) + G(4) + G(3)                                                   \\
       & = \dots                                                                \\
       & = 7c + 6b + 4a                     & = cT(5) + b(T(4) + T(3))  + aT(4) \\
G(7)   & = G(6) + G(5) + G(4)                                                   \\
       & = \dots                                                                \\
       & = 13c + 11b + 7a                   & = cT(6) + b(T(5) + T(4)) + aT(5)  \\
\ldots &                                                                        \\
\end{split}
$$

Thus, CFE for $GT(n)$ can be derived from CFE for $T(n)$.

Using similar techniques, we will be able to identify that
$L = \lim_{n\to\infty} \frac{T(n+1)}{T(n)}$ is one of the 3 roots $\alpha$,
$\beta$, and $\gamma$ of $x^3= x^2 + x + 1$, specifically

$$
L  = \frac
{
1 + \sqrt[3]{19 - 3\sqrt{33}}
+
\sqrt[3]{19 + 3\sqrt{33}}
}
{3}
$$

And $T(n)$ can be computed using the following formula

$$
T(n) =
\frac{\alpha^{n+1}}{(\alpha - \beta)(\alpha -\gamma)}
+
\frac{\beta^{n+1}}{(\beta - \gamma)(\beta -\alpha)}
+
\frac{\gamma^{n+1}}{(\gamma - \alpha)(\gamma -\beta)}
$$

After using the following common property of $\alpha$, $\beta$ and $\gamma$:
$\forall \sigma \text{ satisfies } \sigma^3 = \sigma^2 + \sigma + 1$:

$$
\sigma^{n+1} = \sigma^2(T_n + T_{n-1}) + \sigma(T_n + T_{n-2}) + T_{n-1} + T_{n-2}
$$

(Using $T_n$ notation instead of $T(n)$ to make the equation easier to read.)

See [here](https://mathworld.wolfram.com/TribonacciNumber.html) for more
information on Tribonacci.

## General sums

Given a sequence $G_n$ defined as below:

$$
G_n =
\begin{cases}
a                       & \text{if } n = 0 \\
b                       & \text{if } n = 1 \\
p G_{n-1} + q G_{n-2} & \text{otherwise} \\
\end{cases}
$$

We can prove that

$$
G_n = pF_n + aqF_{n-1} \quad \forall n > 1
$$

With $F_n$ itself is a specialized version of $G_n$ where $a=0$ and $b=1$. Thus,
CFE for $G_n$ can be derived from CFE for $F_n$.

Assuming that $P(x) = x^2 - px - q$ has 2 roots in $\mathbb{R}$

$$
\begin{split}
\alpha & = \frac{p + \sqrt{p^2 + 4q}}{2}              \\
\beta  & = \frac{p - \sqrt{p^2 + 4q}}{2}              \\
\end{split}
$$

We can prove that $x^n = xF_n + qF_{n-1} \forall x \in \{\alpha, \beta\}$, thus:

$$
F_n  = \frac{\alpha^n -  \beta^n}{\alpha - \beta}
      = \frac{\alpha^n -  \beta^n}{\sqrt{p^2 + 4q}}
$$

$F_n$ is known as [Lucas sequence][lucas-seq] (of which _Lucas numbers_ is just
a particular one). The wikipedia link discuss more cases of the CFE for this
sequence, i.e. when $D\le 0$, with $D = p^2+4q$. Also note that even if roots of
$P(x)$ are complex numbers (when $D < 0$), we can still compute $F_n$ using
above formula (I can't prove that, though).

<details>
  <summary>Code to generate Lucas sequence</summary>

```racket
(define a 0)
(define b 1)
(define p 1)
(define q -2)

(define (lucas n)
  (define (iter a b i)
    (if (<= n i) a (iter (+ (* p a) (* q b)) a (+ i 1))))
  (cond
    [(= n 0) a]
    [(= n 1) b]
    [else (iter b a 1)]))

(for ([i (in-range 0 30)])
  (printf "lucas(~a) \t ~a\n" i (lucas i)))
```

</details>

[lucas-seq]: https://en.wikipedia.org/wiki/Lucas_sequence

## More generalizations

After Tribonacci, of course, there is [Tetranacci][fib-4] (4 numbers) and more.
They're known as [_n-Step Fibonacci numbers_][n-fib].

Their limits (called $n$-anacci constant)

$$
L = \lim_{n\to\infty} \frac{F^{n}_{k}}{F^{n}_{k-1}}
$$

is derived by solving

$$
x^n = x^{n-1} + x^{n-2} + \dots + 1
$$

Their formula definitely exist, and should be very, very complicated.

## Closing note

I guess I've over done this exercise. But, I love it. I only know so little and
didn't put much care into the Fibonacci sequence until hitting SICP. Now, I
believe I have refreshed my rusty math knowledge a bit, and learned a few ideas
that hopefully will be useful later.

[n-fib]: https://mathworld.wolfram.com/Fibonaccin-StepNumber.html
[fib-4]: https://mathworld.wolfram.com/TetranacciNumber.html
